\documentclass{ximera}
\input{../preamble.tex}

\title{Exercises} \license{CC BY-NC-SA 4.0}

\begin{document}

\begin{abstract}
\end{abstract}
\maketitle

\begin{onlineOnly}
\section*{Exercises}
\end{onlineOnly}

\begin{problem}\label{exer:2.1.1} Find the general solution.
$$y'+ay=0$$
($a$=constant)
\end{problem}

\begin{problem}\label{exer:2.1.2} Find the general solution.
   $$y'+3x^2y=0$$ 



\begin{solution}
    $\frac{y'}{y}=-3x^2$;\quad $|\ln|y|=-x^3+k$;\quad $y=ce^{-x^3}$.
$y=ce^{-(\ln x)^2/2}$.
\end{solution}
\end{problem}

\begin{problem}\label{exer:2.1.3} Find the general solution.
$$xy'+(\ln x)y=0$$
\end{problem}

\begin{problem}\label{exer:2.1.4} Find the general solution.
$$xy'+3y=0$$



\begin{solution}
    $\frac{y'}{y}=-\frac{3}{x}$;\quad $\ln|y|=-3\ln|x|+k=-\ln|x|^3+k$;\quad
$y=\frac{c}{x^3}$.
\end{solution}
\end{problem}

\begin{problem}\label{exer:2.1.5} Find the general solution.
$$x^2y'+y=0$$ 
\end{problem}

 \begin{problem}\label{exer:2.1.6} Solve
the initial value problem.
$$y'+\left(\frac{1+x}{x}\right)y=0,\quad y(1)=1$$



\begin{solution}
    $\frac{y'}{y}=-\frac{1+x}{x}=-\frac{1}{x}-1$;\quad
$|\ln|y|=-\ln|x|-x+k$;\quad
$y=\frac{ce^{-x}}{x}$;\quad
$y(1)=1\Rightarrow
 c=e$;\quad
$y=\frac{e^{-(x-1)}}{x}$.
\end{solution}
\end{problem}

\begin{problem}\label{exer:2.1.7} Solve
the initial value problem.
$$xy'+\left(1+\frac{1}{\ln x}\right)y=0,\quad y(e)=1$$
\end{problem}

\begin{problem}\label{exer:2.1.8} Solve
the initial value problem.
$$xy'+(1+ x\cot x)y=0,\quad y\left(\frac{\pi}{2}
\right)=2$$



\begin{solution}
    $\frac{y'}{y}=-\frac{1}{x}-\cot x$;
\quad $|\ln|y|=-\ln|x|-\ln|\sin x|+k=-\ln|x\sin x|+k$;\quad
$y=\frac{c}{x\sin x}$;\quad $y(\pi/2)=2\Rightarrow
c=\pi$;\quad $y=\frac{\pi}{x\sin x}$.
\end{solution}
\end{problem}

\begin{problem}\label{exer:2.1.9} Solve
the initial value problem.
$$y'-\left(\frac{2x}{1+x^2}\right)y=0,\quad y(0)=2$$
\end{problem}

\begin{problem}\label{exer:2.1.10} Solve
the initial value problem.
$$y'+\frac{k}{x}y=0,\quad y(1)=3 \quad (k=
\mbox{constant})$$

\begin{solution}
    $\frac{y'}{ y}=-\frac{k}{ x}$;\quad
$\ln|y|=-k\ln|x|+k_1=\ln|x^{-k}|+k_1$;\quad
$y=c|x|^{-k}$;\quad
$y(1)=3\Rightarrow c=3$;\quad $y=3x^{-k}$.
\end{solution}
\end{problem}

\begin{problem}\label{exer:2.1.11} Solve
the initial value problem.
$$y'+(\tan kx)y=0,\quad y(0)=2 \quad (k= \mbox{constant})$$
\end{problem}


\begin{problem}\label{exer:2.1.12} Find
the general solution. 

$$y'+3y=1$$

% A direction field for this equation appears in the GeoGebra interactive below.  Enter the general solution you have found into the equation bar using lower case $c$ as your parameter.  Use the slider to change the value of $c$ to display various particular solutions.

% \begin{center}
% \geogebra{pekp3h7h}{800}{600}
% \end{center}



\begin{solution}
    $\frac{y_1'}{ y_1}=-3$;\quad $\ln|y_1|=-3x$;\quad
$y_1=e^{-3x}$;\quad $y=ue^{-3x}$;\quad
$u'e^{-3x}=1$;\quad $u'=e^{3x}$;\quad $u=\frac{e^{3x}}{3}+c$;\quad
$y=\frac{1}{3}+ce^{-3x}$.
\end{solution}

\end{problem}

\begin{problem}\label{exer:2.1.13} Find
the general solution. 

$$y'+\left(\frac{1}{x}-1\right)y=-\frac{2}{x}$$

% Edit \emph{slopefield1} in the GeoGebra interactive below to plot a direction field on the rectangular region $\{-2\leq x\leq 2,\ -2\leq y\leq 2$\}.  Enter the general solution with lower case $c$ as a parameter to display integral curves.

% \begin{center}
% \geogebra{pekp3h7h}{800}{600}
% \end{center}

\end{problem}

\begin{problem}\label{exer:2.1.14} Find
the general solution. 
$$y'+2xy=xe^{-x^2}$$

% Edit \emph{slopefield1} in the GeoGebra interactive below to plot a direction field on the rectangular region $\{-2\leq x\leq 2,\ -2\leq y\leq 2$\}.  Enter the general solution with lower case $c$ as a parameter to display integral curves.

% \begin{center}
% \geogebra{pekp3h7h}{800}{600}
% \end{center}



\begin{solution}
    $\frac{y_1'}{ y_1}=-2x$;\quad
$\ln|y_1|=-x^2$;\quad
$y_1=e^{-x^2}$;\quad
$y=ue^{-x^2}$;\quad
$u'e^{-x^2}=xe^{-x^2}$;\quad
$u'=x$;\quad
$u=\frac{x^2}{2}+c$;\quad
$y=e^{-x^2}\left(\frac{x^2}{2}+c\right)$.

\end{solution}
\end{problem}

\begin{problem}\label{exer:2.1.15} Find
the general solution. 
$$y'+\frac{2x}{1+x^2}y=\frac{e^{-x}}{1+x^2}$$

% Edit \emph{slopefield1} in the GeoGebra interactive below to plot a direction field on the rectangular region $\{-2\leq x\leq 2,\ -2\leq y\leq 2$\}.  Enter the general solution with lower case $c$ as a parameter to display integral curves.

% \begin{center}
% \geogebra{pekp3h7h}{800}{600}
% \end{center}

\end{problem}

\begin{problem}\label{exer:2.1.16} Find the general solution.
$$y'+\frac{1}{x}y=\frac{7}{x^2}+3$$



\begin{solution}
    $\frac{y_1'}{ y_1}=-\frac{1}{ x}$;\quad
$\ln|y_1|=-\ln|x|$;\quad $y_1=\frac{1}{ x}$;\quad $y=\frac{u}{
x}$;\quad
$\frac{u'}{ x}=\frac{7}{ x^2}+3$;\quad $u'=\frac{7}{
x}+3x$;\quad
$u=7\ln|x|+\frac{3x^2}{2}+c$;\quad $y=\frac{7\ln|x|}{
x}+\frac{3x}{2}+\frac{c}{ x}$.
\end{solution}
\end{problem}


\begin{problem}\label{exer:2.1.17} Find the general solution.
$$y'+\frac{4}{x-1}y= \frac{1}{(x-1)^5}+\frac{\sin x}{(x-1)^4}$$
\end{problem}

\begin{problem}\label{exer:2.1.18} Find the general solution.
$$xy'+(1+2x^2)y=x^3e^{-x^2}$$



\begin{solution}
    $\frac{y_1'}{ y_1}=-\frac{1}{ x}-2x$; \quad
$\ln|y_1|=-\ln|x|-x^2$;\quad $y_1=\frac{e^{-x^2}}{ x}$;\quad
$y=\frac{ue^{-x^2}}{ x}$;\quad
$\frac{u'e^{-x^2}}{ x}=x^2e^{-x^2}$;\quad
 $u'=x^3$;\quad
$u=\frac{x^4}{4}+c$;\quad
$y=e^{-x^2}{\left(\frac{x^3}{4}+\frac{c}{ x}\right)}$.
\end{solution}
\end{problem}

\begin{problem}\label{exer:2.1.19} Find the general solution.
$$xy'+2y=\frac{2}{x^2}+1$$
\end{problem}

\begin{problem}\label{exer:2.1.20} Find the general solution.
$$y'+(\tan x)y=\cos x$$



\begin{solution}
    $\frac{y_1'}{ y_1}=-\tan x$;\quad
$\ln|y_1|=\ln|\cos x|$;\quad
$y_1=\cos x$;\quad $y=u\cos x$;\quad $u'\cos x=\cos x$;\quad
$u'=1$;\quad $u=x+c$;\quad $y=(x+c)\cos x$.
\end{solution}
\end{problem}

\begin{problem}\label{exer:2.1.21} Find the general solution.
$$(1+x)y'+2y=\frac{\sin x}{1 + x}$$
\end{problem}

\begin{problem}\label{exer:2.1.22} Find the general solution.
$$(x-2)(x-1)y'-(4x-3)y=(x-2)^3$$



\begin{solution}
    $\frac{y_1'}{ y_1}=\frac{4x-3}{(x-2)(x-1)}=\frac{5}{
x-2}-\frac{1}{ x-1}$;\quad
$\ln|y_1|=5\ln|x-2|-\ln|x-1|=\ln\left|\frac{(x-2)^5}{
x-1}\right|$;\quad
$y_1=\frac{(x-2)^5}{ x-1}$;\quad
 $y=\frac{u(x-2)^5}{ x-1}$;\quad
$\frac{u'(x-2)^5}{ x-1}=\frac{(x-2)^2}{ x-1}$;\quad
$u'=\frac{1}{ (x-2)^3}$;\quad
$u=-\frac{1}{ 2}\frac{1}{(x-2)^2} +c$;\quad $y=-\frac{1}{
2}\frac{(x-2)^3}{ (x-1)}+c\frac{(x-2)^5}{ (x-1)}$.
\end{solution}
\end{problem}

\begin{problem}\label{exer:2.1.23} Find the general solution.
$$y'+(2\sin x\cos x) y=e^{-\sin^2x}$$
\end{problem}

\begin{problem}\label{exer:2.1.24} Find the general solution.
$$x^2y'+3xy=e^x$$



\begin{solution}
    $\frac{y_1'}{ y_1}=-\frac{3}{ x}$;\quad
$\ln|y_1|=-3\ln|x|=\ln|x|^{-3}$;\quad
$y_1=\frac{1}{ x^3}$;\quad
$y=\frac{u}{ x^3}$;\quad
$\frac{u'}{ x^3}=\frac{e^x}{ x^2}$;\quad
$u'=xe^x$;\quad
$u=xe^x-e^x+c$;\quad
$y=\frac{e^x}{ x^2}-\frac{e^x}{ x^3}+\frac{c}{ x^3}$.
\end{solution}
\end{problem}

\begin{problem}\label{exer:2.1.25} Solve the
initial value problem and sketch the graph of the solution.
$$y'+7y=e^{3x},\quad y(0)=0$$
\end{problem}

\begin{problem}\label{exer:2.1.26} Solve the
initial value problem and sketch the graph of the solution.
$$(1+x^2)y'+4xy=\frac{2}{1+x^2},\quad y(0)=1$$



\begin{solution}
    $\frac{y_1'}{y_1}=-\frac{4x}{1+x^2}$;\quad
$\ln|y_1|=-2\ln(1+x^2)=\ln(1+x^2)^{-2}$;\quad
$y_1=\frac{1}{(1+x^2)^2}$;\quad
$y=\frac{u}{(1+x^2)^2}$;\quad
$\frac{u'}{(1+x^2)^2}=\frac{2}{(1+x^2)^2}$;\quad
$u'=2$;\quad
$u=2x+c$;\quad
$y=\frac{2x+c}{(1+x^2)^2}$;\quad
$y(0)=1\Rightarrow c=1$;\quad
$y=\frac{2x+1}{(1+x^2)^2}$.
\end{solution}
\end{problem}

\begin{problem}\label{exer:2.1.27} Solve the
initial value problem and sketch the graph of the solution.
$$xy'+3y=\frac{2}{x(1+x^2)},\quad y(-1)=0$$
\end{problem}

\begin{problem}\label{exer:2.1.28} Solve the
initial value problem and sketch the graph of the solution.
$$y'+ (\cot x)y=\cos x,\quad
y\left(\frac{\pi}{2}\right)=1$$



\begin{solution}
    $\frac{y_1'}{ y_1}=-\cot x$;\quad
$\ln|y_1|=-\ln|\sin x|$;\quad
$y_1=\frac{1}{\sin x}$;\quad
$y=\frac{u}{\sin x}$;\quad
$\frac{u'}{\sin x}=\cos x$;\quad
$u'=\sin x\cos x$;\quad
$u=\frac{\sin^2x}{2}+c$;\quad
$y=\frac{\sin x}{2}+c\csc x$;\quad
$y(\pi/2)=1\Rightarrow c={1}{2}$;\quad
$y=\frac{1}{2}(\sin x+\csc x)$.
\end{solution}
\end{problem}

\begin{problem}\label{exer:2.1.29} Solve the
initial value problem and sketch the graph of the solution.
$$y'+\frac{1}{x}y=\frac{2}{x^2}+1,\quad y(-1)=0$$
\end{problem}

\begin{problem}\label{exer:2.1.30} Solve the initial value problem.
$$(x-1)y'+3y=\frac{1}{(x-1)^3} +
\frac{\sin x}{(x-1)^2},\quad y(0)=1$$



\begin{solution}
    $\frac{y_1'}{ y_1}=-\frac{3}{ x-1}$;\quad
$\ln|y_1|=-3\ln|x-1|
=\ln|x-1|^{-3}$;\quad
$y_1=\frac{1}{(x-1)^3}$;\quad
$y=\frac{u}{(x-1)^3}$;\quad
$\frac{u'}{(x-1)^3}=
\frac{1}{(x-1)^4}+\frac{\sin
x}{(x-1)^3}$;\quad
$u'=\frac{1}{ x-1}+\sin x$;\quad
$u=\ln|x-1|-\cos x+c$;\quad
$y=\frac{\ln|x-1|-\cos x+c}{(x-1)^3}$;\quad
$y(0)=1\Rightarrow c=0$;\quad
$y=\frac{\ln|x-1|-\cos x}{(x-1)^3}$.
\end{solution}
\end{problem}

\begin{problem}\label{exer:2.1.31} Solve the initial value problem.
$$xy'+2y=8x^2,\quad y(1)=3$$
\end{problem}

\begin{problem}\label{exer:2.1.32} Solve the initial value problem.
$$xy'-2y=-x^2,\quad y(1)=1$$



\begin{solution}
    $\frac{y_1'}{ y_1}=-\frac{2}{ x}$;\quad
$\ln|y_1|=2\ln|x|=\ln(x^2)$;\quad
$y_1=x^2$;\quad
$y=ux^2$;\quad
$u'x^2=-x$;\quad
$u'=-\frac{1}{ x}$;\quad
$u=-\ln|x|+c$;\quad
$y=x^2(c-\ln|x|)$;\quad
$y(1)=1\Rightarrow c=1$;\quad
$y=x^2(1-\ln x)$.
\end{solution}
\end{problem}

\begin{problem}\label{exer:2.1.33} Solve the initial value problem.
$$y'+2xy=x,\quad y(0)=3$$
\end{problem}

\begin{problem}\label{exer:2.1.34} Solve the initial value problem.
$$(x-1)y'+3y=\frac{1+(x-1)\sec^2x}{(x-1)^3},\quad y(0)=-1$$



\begin{solution}
    $\frac{y_1'}{ y_1}=-\frac{3}{ x-1}$;\quad
$\ln|y_1|=-3\ln|x-1|=\ln|x-1|^{-3}$;\quad
$y_1=\frac{1}{(x-1)^3}$;\quad
$y=\frac{u}{(x-1)^3}$;\quad
$\frac{u'}{(x-1)^3}=\frac{1+(x-1)\sec^2x}{(x-1)^4}$;\quad
$u'=\frac{1}{ x-1}+\sec^2x$;\quad
$u=\ln|x-1|+\tan x+c$;\quad
$y=\frac{\ln|x-1|+\tan x+c}{(x-1)^3}$;\quad
$y(0)=-1\Rightarrow c=1$;\quad
$y=\frac{\ln|x-1|+\tan
x+1}{(x-1)^3}$.
\end{solution}
\end{problem}

\begin{problem}\label{exer:2.1.35} Solve the initial value problem.
$$(x+2)y'+4y=\frac{1+2x^2}{x(x+2)^3},\quad y(-1)=2$$
\end{problem}

\begin{problem}\label{exer:2.1.36} Solve the initial value problem.
$$(x^2-1)y'-2xy=x(x^2-1),\quad y(0)=4$$



\begin{solution}
    $\frac{y_1'}{ y_1}=\frac{2x}{ x^2-1}$;\quad
$\ln|y_1|=\ln|x^2-1|$;\quad
$y_1=x^2-1$;\quad
$y=u(x^2-1)$;\quad
$u'(x^2-1)=x$;\quad
$u'=\frac{x}{ x^2-1}$;\quad
$u=\frac{1}{2}\ln|x^2-1|+c$;\quad
$y=(x^2-1)\left(\frac{1}{2}\ln|x^2-1|+c\right)$;\quad
$y(0)=4\Rightarrow c=-4$;\quad
$y=(x^2-1)\left(\frac{1}{2}\ln|x^2-1|-4\right)$.
\end{solution}
\end{problem}

\begin{problem}\label{exer:2.1.37} Solve the initial value problem.
$$(x^2-5)y'-2xy=-2x(x^2-5),\quad y(2)=7$$
\end{problem}

\begin{problem}\label{exer:2.1.38} Solve the initial value problem and leave the answer in a form involving a definite integral.
$$y'+2xy=x^2,\quad y(0)=3$$



\begin{solution}
    $\frac{y_1'}{ y_1}=-2x$;\quad
$\ln|y_1|=-x^2$;\quad
$y_1=e^{-x^2}$;\quad
$y=ue^{-x^2}$;\quad
$u'e^{-x^2}=x^2$;\quad
$u'=x^2e^{x^2}$;\quad
$u=c+{\int_0^xt^2e^{t^2}\,dt}$;\quad
$y=e^{-x^2}\left(c+{\int_0^xt^2e^{t^2}\,dt}\right)$;\quad
$y(0)=3\Rightarrow c=3$;\quad
$y=e^{-x^2}\left(3+{\int_0^xt^2e^{t^2}\,dt}\right)$.

\end{solution}
\end{problem}

\begin{problem}\label{exer:2.1.39} Solve the initial value problem and leave the answer in a form involving a definite integral.
$$y'+\frac{1}{x}y=\frac{\sin x}{x^2},\quad y(1)=2$$
\end{problem}

\begin{problem}\label{exer:2.1.40} Solve the initial value problem and leave the answer in a form involving a definite integral.
$$y'+y=\frac{e^{-x}\tan x}{x},\quad y(1)=0$$



\begin{solution}
    $\frac{y_1'}{ y_1}=-1$;\quad
$\ln|y_1|=-x$;\quad
$y_1=e^{-x}$;\quad
$y=ue^{-x}$;\quad
$u'e^{-x}=\frac{e^{-x}\tan x}{ x}$;\quad
$u'=\frac{\tan x}{ x}$;\quad
$u=c+\int_1^x\frac{\tan t}{ t}\,dt$;\quad
$y=e^{-x}\left(c+\int_1^x\frac{\tan t}{ t}\,dt\right)$;\quad
$y(1)=0\Rightarrow c=0$;\quad
$y=e^{-x}\int_1^x\frac{\tan t}{ t}\,dt$.
\end{solution}
\end{problem}

\begin{problem}\label{exer:2.1.41} Solve the initial value problem and leave the answer in a form involving a definite integral.
$$y'+\frac{2x}{1+x^2}y=\frac{e^x}{(1+x^2)^2}, \quad y(0)=1$$
\end{problem}

\begin{problem}\label{exer:2.1.42} Solve the initial value problem and leave the answer in a form involving a definite integral.
$$xy'+(x+1)y=e^{x^2},\quad y(1)=2$$



\begin{solution}
    $\frac{y_1'}{ y_1}=-1-\frac{1}{ x}$;\quad
$\ln|y_1|=-x-\ln|x|$;\quad
$y_1=\frac{e^{-x}}{ x}$;\quad
$y=\frac{ue^{-x}}{ x}$;\quad
$\frac{u'e^{-x}}{ x}=\frac{e^{x^2}}{ x}$;\quad
$u'=e^xe^{x^2}$;\quad
$u=c+\int_1^xe^te^{t^2}\,dt$;\quad
$y=\frac{e^{-x}}{ x}\left(c+\int_1^xe^te^{t^2}\,dt\right)$;\quad
$y(1)=2\Rightarrow c=2e$;\quad
$y=\frac{1}{x}\left(2e^{-(x-1)}+e^{-x}\int_1^xe^te^{t^2}\,dt\right)$.
\end{solution}
\end{problem}

\begin{problem}\label{exer:2.1.43}
Experiments indicate that glucose is absorbed by the body at a rate proportional to the amount of glucose present in the bloodstream. Let $\lambda$ denote the (positive) constant of proportionality. Now suppose glucose is injected into a patient's bloodstream at a constant rate of $r$ units per unit of time. Let $G=G(t)$ be the number of units in the patient's bloodstream at time $t>0$. Then
$$G'=-\lambda G+r$$
where the first term on the right is due to the absorption of the glucose by the patient's body and the second term is due to the injection. Determine $G$ for $t>0$, given that $G(0)=G_0$. Also, find $\lim_{t\to\infty}G(t)$.
\end{problem}

\begin{problem}\label{exer:2.1.44}
\begin{enumerate}
\item % (a)
Plot a direction field and some integral curves for
\begin{equation}\label{eqA:2.1.44}
    xy'-2y=-1
\end{equation}
on the rectangular region  $\{-1\leq x\leq 1, -.5\leq y\leq 1.5\}$.
What do all the integral curves have in common?

\item \label{part2.1.44b}%(b)
Show that the general solution of (\ref{eqA:2.1.44})
on $(-\infty,0)$ and $(0,\infty)$ is
$$
y=\frac{1}{2}+cx^2.
$$



\begin{solution}
    Eqn. (\ref{eqA:2.1.44}) is equivalent to
$$
y'-\frac{2}{ x}=-\frac{1}{ x}
$$
on $(-\infty,0)$ and $(0,\infty)$. Here
$\frac{y_1'}{ y_1}=\frac{2}{ x}$;\quad $\ln|y_1|=2\ln|x|$;\quad
$y_1=x^2$;\quad
$y=ux^2$;\quad $u'x^2=-\frac{1}{ x}$;\quad $u'=-\frac{1}{
x^3}$;\quad
$u=\frac{1}{2x^2}+c$, so $y=\frac{1}{2}+cx^2$ is the general
solution of (\ref{eqA:2.1.44}) on $(-\infty,0)$ and $(0,\infty)$.
\end{solution}

\item % (c)
Show that $y$ is a solution of (\ref{eqA:2.1.44}) on
$(-\infty,\infty)$ if and only if
$$
y=\left\{\begin{array}{ll}0.5+c_1x^2, &x
\ge 0,\\
0.5+c_2x^2, &x < 0,\end{array}\right.
$$
 where $c_1$ and $c_2$ are arbitrary constants.

 

 \begin{solution}
     From the proof of (b), any solution of (\ref{eqA:2.1.44}) must be of the form
$$
y=\left\{\begin{array}{ll}\frac{1}{2}+c_1x^2, &x
\ge 0,\\
\frac{1}{2}+c_2x^2, &x < 0,\end{array}\right.
$$
for $x\ne0$, and any function of this form
satisfies (\ref{eqA:2.1.44}) for $x\ne0$. To complete the proof we
must show that any function of this form is
differentiable and satisfies (\ref{eqA:2.1.44}) at $x=0$. By
definition,
$$
y'(0)=\lim_{x\to0}\frac{y(x)-y(0)}{ x-0}=\lim_{x\to0}\frac{y(x)-1/2}{
x}
$$
if the limit exists. But
$$
\frac{y(x)-1/2}{ x}=\left\{\begin{array}{cl} c_1x,&x>0\\
c_2x,&x<0,\end{array}\right.
$$
so $y'(0)=0$. Since $0y'(0)-2y(0)=0\cdot0-2(1/2)=-1$, any function of
this form satisfies (\ref{eqA:2.1.44}) at
$x=0$.
 \end{solution}

\item % (d)
Conclude that all solutions of (\ref{eqA:2.1.44}) on
$(-\infty,\infty)$ are solutions of the initial value problem
$$
xy'-2y=-1,\quad y(0)=\frac{1}{2}.
$$

Click below to see the solution.

\begin{solution}
    From (b) any solution $y$ of (\ref{eqA:2.1.44}) on
$(-\infty,\infty)$ is of the form
$$
y=\left\{\begin{array}{ll}\frac{1}{2}+c_1x^2, &x
\ge 0,\\
\frac{1}{2}+c_2x^2, &x < 0,\end{array}\right.
$$
So,
$y(0)=1/2$.
\end{solution}

\item %(e)
Use part \ref{part2.1.44b} to show that if  $x_0\neq 0$ and $y_0$  is arbitrary, then
  the  initial value problem
$$
xy'-2y=-1,\quad y(x_0)=y_0
$$
has infinitely many solutions on ($-\infty,\infty$). Explain why this
doesn't contradict  Theorem~\ref{thmtype:2.1.1}(b).



\begin{solution}
    If $x_0>0$, then every function of the form
$$
y=\left\{\begin{array}{ll}\frac{1}{2}+c_1x^2, &x
\ge 0,\\
\frac{1}{2}+c_2x^2, &x < 0,\end{array}\right.
$$
with $c_1=\frac{y_0-1/2}{x_0^2}$ and $c_2$
arbitrary is a solution of the initial value problem on
$(-\infty,\infty)$. Since these functions are all identical on
$(0,\infty)$, this does not contradict Theorem~2.1.1, which
implies that 
$y'-\frac{2}{x}=-\frac{1}{x}$ (so
(\ref{eqA:2.1.44})) has exactly one solution on $(0,\infty)$ such
that $y(x_0)=y_0$. A similar argument applies if $x_0<0$.
\end{solution}
\end{enumerate}
\end{problem}

\begin{problem}\label{exer:2.1.45}
Suppose $f$ is continuous on an open interval $(a,b)$
and $\alpha$ is a constant.
\begin{enumerate}
\item %(a)
Derive a formula for the solution of the initial value
problem

\begin{equation}\label{eqA:2.1.45}
y'+\alpha y=f(x),\quad y(x_0)=y_0
\end{equation}
where $x_0$ is in $(a,b)$ and $y_0$ is an arbitrary real number.

\item %(b)
Suppose $(a,b)=(a,\infty)$, $\alpha > 0$ and
$\lim_{x\to\infty} f(x)=L$. Show that if $y$ is the
solution of (\ref{eqA:2.1.45}), then $\lim_{x\to
\infty y(x)=L/\alpha}$.
\end{enumerate}
\end{problem}

\begin{problem}\label{exer:2.1.46}
Assume that all functions in this exercise are defined on
a common interval $(a,b)$.
\begin{enumerate}
\item %(a)
Prove:  If $y_1$ and $y_2$ are solutions of
$$
y'+p(x)y=f_1(x)
$$
and
$$
y'+p(x)y=f_2(x)
$$
respectively, and $c_1$ and $c_2$ are constants, then
$y=c_1y_1+c_2y_2$ is a solution of
$$
y'+p(x)y=c_1f_1(x)+c_2f_2(x).
$$
(This is the \emph{principle of superposition}.)



\begin{solution}
    Let $y=c_1y_1+c_2y_2$. Then
\begin{eqnarray*}
y'+p(x)y&=&(c_1y_1+c_2y_2)'+p(x)(c_1y_1+c_2y_2)\\
&=&c_1y_1'+c_2y_2'+c_1p(x)y_1+c_2p(x)y_2\\
&=&c_1(y_1'+p(x)y_1)+c_2(y_2+p(x)y_2)=c_1f_1(x)+c_2f_2(x).
\end{eqnarray*}
\end{solution}

\item %(b)
Use the previous part to show that if $y_1$ and $y_2$ are solutions
of the nonhomogeneous equation
\begin{equation}\label{eqA:2.1.46}
y'+p(x)y=f(x)
\end{equation}
then $y_1-y_2$ is a solution of the homogeneous equation
\begin{equation}\label{eqB:2.1.46}
y'+p(x)y=0.
\end{equation}



\begin{solution}
    Let $f_1=f_2=f$ and $c_1=-c_2=1$.
\end{solution}

\item %(c)
Show that if $y_1$ is a solution of
(\ref{eqA:2.1.46}) and $y_2$ is a solution of
(\ref{eqB:2.1.46}), then $y_1+y_2$ is a solution of
(\ref{eqA:2.1.46}).



\begin{solution}
    Let $f_1=f$, $f_2=0$, and $c_1=c_2=1$.
\end{solution}
\end{enumerate}
\end{problem}

\begin{problem}\label{exer:2.1.47}
Some nonlinear equations can be transformed into linear
equations by changing the dependent variable.  Show that if
$$
g'(y)y'+p(x)g(y)=f(x)
$$
where $y$ is a function of $x$ and $g$ is a function of $y$,
then the new dependent variable $z=g(y)$ satisfies the
linear equation
$$
z'+p(x)z=f(x).
$$
\end{problem}

\begin{problem}\label{exer:2.1.48}
Solve by the method discussed in Exercise~\ref{exer:2.1.47}.

\begin{enumerate} 
\item 
$(\sec^2y)y'- 3\tan y=-1$



\begin{solution}
    If $z=\tan y$, then $z'=(\sec^2y)y'$, so $z'-3z=-1$;\;
$z_1=e^{3x}$;\;
$z=ue^{3x}$;\;
$u'e^{3x}=-1$;\;
$u'=-e^{-3x}$;\;
$u=\frac{e^{-3x}}{3}+c$;\;
$z=\frac{1}{3}+ce^{3x}=\tan y$;\;
$y=\tan^{-1}\left(\frac{1}{3}+ce^{3x}\right)$.
\end{solution}

\item 
$e^{y^2}\left(2yy'+\frac{2}{x}\right) =\frac{1}{x^2}$



\begin{solution}
    If $z=e^{y^2}$, then $z'=2yy'e^{y^2}$, so $z'+\frac{2}{
x}z=\frac{1}{ x^2}$;\;
$z_1=\frac{1}{ x^2}$;\;
$z=\frac{u}{ x^2}$;\;
$\frac{u'}{ x^2}=\frac{1}{ x^2}$;\;
$u'=1$;\;
$u=x+c$;\;
$z=\frac{1}{ x}+\frac{c}{ x^2}=e^{y^2}$;\;
$y=\pm\left[\ln\left(\frac{1}{ x}+\frac{c}{
x^2}\right)\right]^{1/2}$.
\end{solution}

\item 
$\frac{xy'}{y} + 2\ln y=4x^2$



\begin{solution}
    Rewrite the equation as $\frac{y'}{ y}+\frac{2}{ x}\ln y=4x$.
If $z=\ln y$, then $z'=\frac{y'}{ y}$, so $z'+\frac{2}{ x}z=4x$;
\
$z_1=\frac{1}{ x^2}$;\;
$z=\frac{u}{ x^2}$;\;
$\frac{u'}{ x^2}=4x$;\;
$u'=4x^3$;\;
$u=x^4+c$;\;
$z=x^2+\frac{c}{ x^2}=\ln y$;\;
$y=\exp\left(x^2+\frac{c}{ x^2}\right)$.
\end{solution}

\item 
$\frac{y'}{(1+y)^2} -\frac{1}{x(1+y)}=-\frac{3}{x^2}$



\begin{solution}
    If $z=-\frac{1}{ 1+y}$, then $z'=\frac{y'}{(1+y)^2}$, so
$z'+\frac{1}{ x}z=-\frac{3}{ x^2}$;\;
$z_1=\frac{1}{ x}$;\;
$z=\frac{u}{ x}$;\;
$\frac{u'}{ x}=-\frac{3}{ x^2}$;\;
$u'=-\frac{3}{ x}$;\;
$u=-3\ln|x|-c$;\;
$z=-\frac{3\ln|x|+c}{ x}=-\frac{1}{1+y}$;\;
$y=-1+\frac{x}{3\ln|x|+c}$.
\end{solution}
\end{enumerate}
\end{problem}

\begin{problem}\label{exer:2.1.49}
We've shown that if $p$ and $f$ are continuous on $(a,b)$
then every solution of
\begin{equation}\label{eqA:2.1.49}
y'+p(x)y=f(x)
\end{equation}
on $(a,b)$ can be written as $y=uy_1$, where
$y_1$ is a nontrivial solution of the complementary equation for (\ref{eqA:2.1.49})
and $u'=f/y_1$. Now suppose   $f$, $f'$, \dots, $f^{(m)}$ and
$p$, $p'$, \dots, $p^{(m-1)}$ are continuous on $(a,b)$, where $m$
is a positive integer, and define
\begin{eqnarray*}
f_0&=&f,\\ f_j&=&f_{j-1}'+pf_{j-1},\quad 1\leq j\leq m.
\end{eqnarray*}
Show that
$$
u^{(j+1)}=\frac{f_j}{y_1},\quad 0\leq j\leq m.
$$
\end{problem}

\end{document}